LambdaS5/coq/LjsRulesCorrectCall.v
@@ -1,0 +1,726 @@
+Generalizable All Variables.
+Set Implicit Arguments.
+Require Import JsNumber.
+Require Import LjsShared.
+Require Import Utils.
+Require Import LjsRulesCorrectDefinitions.
+Require Import LjsRulesCorrectCommon.
+Require Import LjsRulesCorrectSpecFuns.
+Require Import LjsRulesCorrectCallPrealloc.
+Import ListNotations.
+Open Scope list_scope.
+Open Scope string_scope.
+
+Implicit Type A B : Type.
+Implicit Type s : string.
+Implicit Type n : number.
+Implicit Type i : L.id.
+Implicit Type st : L.store.
+Implicit Type e : L.expr.
+Implicit Type v : L.value.
+Implicit Type o : L.out.
+Implicit Type c : L.ctx.
+Implicit Type ptr : L.object_ptr.
+Implicit Type obj : L.object.
+Implicit Type re : L.result.
+Implicit Type r : L.res.
+Implicit Type props : L.object_props.
+
+Implicit Type jst : J.state.
+Implicit Type je : J.expr.
+Implicit Type jt : J.stat.
+Implicit Type jee : J.ext_expr.
+Implicit Type jet : J.ext_stat.
+Implicit Type jes : J.ext_spec.
+Implicit Type jc : J.execution_ctx.
+Implicit Type jo : J.out.
+Implicit Type jr : J.res.
+Implicit Type jv : J.value.
+Implicit Type jptr : J.object_loc.
+Implicit Type jobj : J.object.
+Implicit Type jrv : J.resvalue.
+Implicit Type jref : J.ref.
+Implicit Type jl : J.label.
+Implicit Type jer : J.env_record.
+Implicit Type jeptr : J.env_loc.
+Implicit Type jder : J.decl_env_record.
+Implicit Type jprops : J.object_properties_type.
+Implicit Type jlenv : J.lexical_env.
+
+Lemma binding_inst_formal_params_lemma_lemma : forall BR k jst jc c st st' r is vs jvs1 jvs2 ptr ptr1 jeptr b k',
+    L.red_exprh k c st (L.expr_basic (L.expr_seqs_then L.expr_empty
+            (map E.init_arg (zipl_stream (LibStream.map string_of_nat (nat_stream_from k')) is)))) 
+        (L.out_ter st' r) ->
+    context_invariant BR jc c ->
+    state_invariant BR jst st ->
+    values_related BR (jvs1 ++ jvs2) vs ->
+    k' = length jvs1 /\ length jvs2 > 0 \/ k' >= length jvs1 /\ jvs2 = [] ->
+    binds c "$strict" (L.value_bool b) ->
+    binds c "$vcontext" (L.value_object ptr) ->
+    binds c "args" (L.value_object ptr1) ->
+    fact_iarray ptr1 vs \in BR ->
+    fact_js_env jeptr ptr \in BR ->
+    concl_ext_expr_resvalue BR jst jc c st st' r 
+        (J.spec_binding_inst_formal_params jvs2 jeptr is b) (fun jrv => jrv = J.resvalue_empty).    
+Proof.
+    introv.
+    unfolds E.init_args.
+    inductions is gen BR k jst st jvs1 jvs2;
+    introv Hlred Hcinv Hinv Hvrels Hk' Hbinds1 Hbinds2 Hbinds3 Hf1 Hf2. {
+        repeat ljs_autoforward.
+        jauto_js 10.
+    }
+    simpl in Hlred.
+    rew_map in Hlred.
+    repeat ljs_autoforward.
+    forwards_th Harridx : array_idx_lemma. reflexivity. eassumption. eassumption.
+    destruct Harridx as (?&Heq1&jv&v&Heq2&Hvrel&Harridx). subst_hyp Heq1. subst_hyp Heq2.
+    asserts Hjvs2 : (k' >= length jvs1 /\ jvs2 = [] /\ v = L.value_undefined /\ jv = J.value_prim J.prim_undef \/ 
+            k' = length jvs1 /\ exists jvs2', jvs2 = jv::jvs2'). {
+        destruct Hk' as [(Hk1&Hk2)|(Hk1&Hk2)]. {
+            right. split. assumption. 
+            destruct jvs2; rew_length in Hk2; try solve [false; math].
+            destruct Harridx as [Harridx|Harridx]. {
+                erewrite <- values_related_length_lemma in Harridx by eassumption.
+                rew_length in Harridx. destruct_hyp Harridx. false. math.
+            }
+            destruct Harridx as (Harridx1&Harridx2).
+            apply Nth_app_inv in Harridx1.
+            destruct Harridx1 as [Harridx1|Harridx1]. {
+                apply Nth_lt_length in Harridx1. false. math.
+            }
+            destruct Harridx1 as (k''&Heqk''&Harridx1).
+            asserts Hzero : (k'' = 0). { math. } subst_hyp Hzero.
+            inverts Harridx1.
+            jauto.
+        } {
+            left. 
+            destruct Harridx as [Harridx|Harridx]. {
+                destruct_hyp Harridx. jauto.
+            }
+            subst_hyp Hk2.
+            destruct Harridx as (Harridx1&Harridx2).
+            rew_app in Harridx1.
+            apply Nth_lt_length in Harridx1. false. math.
+        }
+    }
+    clear Harridx. clear Hk'.
+    asserts Hexit : (exists jvs1' jvs2', values_related BR (jvs1' ++ jvs2') vs /\
+            (S k' = length jvs1' /\ length jvs2' > 0 \/ S k' >= length jvs1' /\ jvs2' = []) /\
+            (k' >= length jvs1 /\ jvs2 = [] /\ v = L.value_undefined /\ jv = J.value_prim J.prim_undef /\
+                jvs1' = jvs1 /\ jvs2' = jvs2 \/ 
+             k' = length jvs1 /\ jvs1' = jvs1 & jv /\ jvs2 = jv::jvs2')). {
+        destruct Hjvs2 as [Hjvs2|Hjvs2]. {
+            exists jvs1 jvs2.
+            destruct_hyp Hjvs2. splits. 
+            + assumption. 
+            + right. split. math. reflexivity.
+            + left. jauto_js.
+        } {
+            destruct_hyp Hjvs2. destruct jvs2' as [|jv' jvs2']. {
+                exists (jvs1&jv) (@nil J.value). splits.
+                + rew_app. assumption.
+                + right. split. { rew_length. math. } reflexivity.
+                + right. jauto_js.
+            }
+            exists (jvs1&jv) (jv'::jvs2'). splits. 
+            + rew_app. assumption.
+            + left. split. { rew_length. math. } { rew_length. math. }
+            + right. jauto_js.
+        }
+    }
+    repeat ljs_autoforward.
+    inverts red_exprh H3. (* TODO *)
+    ljs_apply.
+    ljs_context_invariant_after_apply.
+    repeat ljs_autoforward.
+    forwards_th: has_binding_lemma. prove_bag.
+    destr_concl; [idtac | destruct_hyp Hjvs2; try ljs_handle_abort].
+    res_related_invert.
+    resvalue_related_invert.
+    repeat ljs_autoforward.
+    destruct b0. { (* binding already exists *)
+        repeat ljs_autoforward.
+        forwards_th: set_mutable_binding_lemma. prove_bag.
+        destr_concl; [idtac | destruct_hyp Hjvs2; try ljs_handle_abort].
+        res_related_invert.
+        resvalue_related_only_invert.
+        repeat ljs_autoforward.
+        destruct Hexit as (jvs1'&jvs2'&Hvrels'&Hsk'&Hjvs2').
+        forwards_th Hx : IHis; try prove_bag. eauto_js.
+        destr_concl; [idtac | destruct_hyp Hjvs2'; try ljs_handle_abort].
+        destruct_hyp Hjvs2'; jauto_js 10.
+    } { (* binding does not exist *)
+        repeat ljs_autoforward.
+        forwards_th: create_mutable_binding_lemma_none. prove_bag.
+        destr_concl; [idtac | destruct_hyp Hjvs2; try ljs_handle_abort].
+        res_related_invert.
+        resvalue_related_only_invert.
+        repeat ljs_autoforward.
+        forwards_th: set_mutable_binding_lemma. prove_bag.
+        destr_concl; [idtac | destruct_hyp Hjvs2; try ljs_handle_abort]. 
+        res_related_invert.
+        resvalue_related_only_invert.
+        repeat ljs_autoforward.
+        destruct Hexit as (jvs1'&jvs2'&Hvrels'&Hsk'&Hjvs2').
+        forwards_th Hx : IHis; try prove_bag. eauto_js.
+        destr_concl; [idtac | destruct_hyp Hjvs2'; try ljs_handle_abort].
+        destruct_hyp Hjvs2'; jauto_js 10.
+    }
+Qed.
+
+Lemma binding_inst_formal_params_lemma : forall BR k jst jc c st st' r is vs jvs ptr ptr1 jeptr b,
+    L.red_exprh k c st (L.expr_basic (E.init_args is)) (L.out_ter st' r) ->
+    context_invariant BR jc c ->
+    state_invariant BR jst st ->
+    values_related BR jvs vs ->
+    binds c "$strict" (L.value_bool b) ->
+    binds c "$vcontext" (L.value_object ptr) ->
+    binds c "args" (L.value_object ptr1) ->
+    fact_iarray ptr1 vs \in BR ->
+    fact_js_env jeptr ptr \in BR ->
+    concl_ext_expr_resvalue BR jst jc c st st' r 
+        (J.spec_binding_inst_formal_params jvs jeptr is b) (fun jrv => jrv = J.resvalue_empty).    
+Proof.
+    introv Hlred Hcinv Hinv Hvrels Hbinds1 Hbinds2 Hbinds3 Hf1 Hf2.
+    asserts Hvrels' : (values_related BR ([]++jvs) vs). { rew_app. assumption. }
+    forwards_th : binding_inst_formal_params_lemma_lemma; try prove_bag.
+    destruct jvs; rew_length; intuition math.
+Qed.
+
+Lemma binding_inst_arg_obj_lemma : forall BR k jst jc c st st' r jptr ptr ptr1 ptr2(*ptr3*)is jvs vs jeptr jlenv v b,
+    L.red_exprh k c st (L.expr_app_2 LjsInitEnv.privEnvDefineArgsObjOk
+        [L.value_object ptr2; L.value_null(*object ptr3*); L.value_object ptr1; L.value_object ptr; L.value_bool b]) 
+        (L.out_ter st' r) ->
+    context_invariant BR jc c ->
+    state_invariant BR jst st ->
+    values_related BR jvs vs ->
+    lexical_env_related BR jlenv v ->
+    fact_js_obj jptr ptr \in BR ->
+    fact_iarray ptr1 vs \in BR ->
+(*    fact_iarray ptr3 (map L.value_string is) \in BR -> TODO non-strict args obj *)
+    fact_js_env jeptr ptr2 \in BR ->
+    fact_ctx_parent ptr2 v \in BR ->
+    J.execution_ctx_variable_env jc = jeptr::jlenv ->
+    concl_ext_expr_resvalue BR jst jc c st st' r 
+        (J.spec_binding_inst_arg_obj jptr is jvs jeptr b) (fun jrv => jrv = J.resvalue_empty).
+Proof.
+    introv Hlred Hcinv Hinv Hvrel Hlrel Hf1 Hf2 Hf3 Hf4 Hvenv.
+    inverts red_exprh Hlred.
+    ljs_apply.
+    ljs_context_invariant_after_apply.
+    repeat ljs_autoforward.
+    forwards_th Hx : create_arguments_object_ok; try prove_bag.
+    rewrite <- Hvenv in Hx.
+    destr_concl; try ljs_handle_abort.
+    res_related_invert.
+    resvalue_related_only_invert.
+    repeat ljs_autoforward.
+    destruct b. { (* strict *)
+        repeat ljs_autoforward.
+        forwards_th : create_immutable_binding_lemma. prove_bag.
+        destr_concl; try ljs_handle_abort.
+        res_related_invert.
+        repeat ljs_autoforward.
+        forwards_th : initialize_immutable_binding_lemma. prove_bag.
+        destr_concl; try ljs_handle_abort.
+        res_related_invert.
+        resvalue_related_only_invert.
+        jauto_js 10.
+    } { (* non-strict *)
+        repeat ljs_autoforward.
+        forwards_th : create_set_mutable_binding_lemma_none. prove_bag.
+        destr_concl; try ljs_handle_abort.
+        res_related_invert.
+        resvalue_related_only_invert.
+        jauto_js 10.
+    }
+Qed.
+
+Lemma binding_inst_function_decls_lemma : forall BR k jst jc c st st' r jfds jeptr ptr b1 b2,
+    L.red_exprh k c st (L.expr_basic 
+        (E.init_funcs b1 E.make_fobj (map E.js_funcdecl_to_func jfds))) (L.out_ter st' r) ->
+    context_invariant BR jc c ->
+    state_invariant BR jst st ->
+    binds c "$strict" (L.value_bool b2) ->
+    binds c "$vcontext" (L.value_object ptr) ->
+    fact_js_env jeptr ptr \in BR ->
+    concl_ext_expr_resvalue BR jst jc c st st' r 
+        (J.spec_binding_inst_function_decls jeptr jfds b2 b1) (fun jrv => jrv = J.resvalue_empty).    
+Proof.
+    introv.
+    unfolds E.init_funcs.
+    inductions jfds gen BR k jst st;
+    introv Hlred Hcinv Hinv Hbinds1 Hbinds2 Hf. {
+        repeat ljs_autoforward.
+        jauto_js.
+    }
+    destruct a. destruct funcdecl_body.
+    rew_map in Hlred.
+    repeat ljs_autoforward.
+    rewrite exprjs_prog_strictness_eq in *.
+    forwards_th : red_spec_creating_function_object_ok. skip. (* { TODO in ES5 variable env required, fixed in ES6
+        introv Hbinds.
+        binds_inv.
+        applys (execution_ctx_related_lexical_env (context_invariant_execution_ctx_related Hcinv)).
+        assumption.
+    } *)
+    destr_concl; try ljs_handle_abort.
+    res_related_invert.
+    resvalue_related_invert.
+    repeat ljs_autoforward.
+    inverts red_exprh H12. (* TODO *)
+    ljs_apply.
+    ljs_context_invariant_after_apply.
+    repeat ljs_autoforward.
+    forwards_th: has_binding_lemma. prove_bag.
+    destr_concl; try ljs_handle_abort.
+    res_related_invert.
+    resvalue_related_invert.
+    repeat ljs_autoforward.
+    destruct b. { (* binding already exists *)
+        repeat ljs_autoforward.
+        cases_decide as Hgctx. { (* on global context *)
+            skip. (* TODO global context *)
+        }
+        asserts Hq : (jeptr <> J.env_loc_global_env_record). {
+            unfolds LjsInitEnv.privglobalContext.
+            rewrite stx_eq_object_eq_lemma in Hgctx.
+            forwards Hger : context_invariant_global_env_record_lemma Hcinv.
+            intro Hjeptr. subst_hyp Hjeptr. apply Hgctx.
+            determine_fact_js_env.
+            reflexivity.
+        }
+        repeat ljs_autoforward.
+        forwards_th: set_mutable_binding_lemma. prove_bag.
+        destr_concl; try ljs_handle_abort.
+        res_related_invert.
+        repeat ljs_autoforward.
+        forwards_th : IHjfds; try prove_bag.
+        destr_concl; try ljs_handle_abort.
+        res_related_invert.
+        jauto_js 10.
+    } { (* binding does not exist *)
+        repeat ljs_autoforward.
+        forwards_th: create_mutable_binding_lemma_some. prove_bag.
+        destr_concl; try ljs_handle_abort.
+        res_related_invert.
+        repeat ljs_autoforward.
+        forwards_th: set_mutable_binding_lemma. prove_bag.
+        destr_concl; try ljs_handle_abort.
+        res_related_invert.
+        resvalue_related_only_invert.
+        repeat ljs_autoforward.
+        forwards_th : IHjfds; try prove_bag.
+        destr_concl; try ljs_handle_abort.
+        res_related_invert.
+        jauto_js 10.
+    }
+Qed.
+
+Lemma binding_inst_var_decls_lemma : forall BR k jst jc c st st' r is jeptr ptr b1 b2,
+    L.red_exprh k c st (L.expr_basic (E.init_vars b1 is)) (L.out_ter st' r) ->
+    context_invariant BR jc c ->
+    state_invariant BR jst st ->
+    binds c "$strict" (L.value_bool b2) ->
+    binds c "$vcontext" (L.value_object ptr) ->
+    fact_js_env jeptr ptr \in BR ->
+    concl_ext_expr_resvalue BR jst jc c st st' r 
+        (J.spec_binding_inst_var_decls jeptr is b1 b2) (fun jrv => jrv = J.resvalue_empty).
+Proof.
+    introv.
+    unfolds E.init_vars.
+    inductions is gen BR k jst st;
+    introv Hlred Hcinv Hinv Hbinds1 Hbinds2 Hf. {
+        repeat ljs_autoforward.
+        jauto_js.
+    }
+    rew_map in Hlred.
+    repeat ljs_autoforward.
+    inverts red_exprh H3.
+    ljs_apply.
+    ljs_context_invariant_after_apply.
+    repeat ljs_autoforward.
+    forwards_th: has_binding_lemma. eassumption.
+    destr_concl; try ljs_handle_abort.
+    res_related_invert.
+    resvalue_related_invert.
+    repeat ljs_autoforward.
+    destruct b. { (* binding already exists *)
+        repeat ljs_autoforward.
+        forwards_th : IHis; try prove_bag.
+        destr_concl; try ljs_handle_abort.
+        res_related_invert.
+        jauto_js 10.
+    } { (* binding does not exist *)
+        repeat ljs_autoforward.
+        forwards_th: create_set_mutable_binding_lemma_some. prove_bag.
+        destr_concl; try ljs_handle_abort.
+        res_related_invert.
+        repeat ljs_autoforward.
+        forwards_th : IHis; try prove_bag.
+        destr_concl; try ljs_handle_abort.
+        res_related_invert.
+        jauto_js 10.
+    }
+Qed.
+
+Opaque E.init_args E.init_vars E.init_funcs.
+
+Lemma binding_inst_global_lemma : forall BR k jst jc c st st' r ptr jp,
+    L.red_exprh k c st (L.expr_basic
+          (E.init_bindings_prog false E.make_fobj (concat (List.map E.js_element_to_func (J.prog_elements jp))) 
+              (J.prog_vardecl jp))) (L.out_ter st' r) ->
+    context_invariant BR jc c ->
+    state_invariant BR jst st ->
+    binds c "$strict" (L.value_bool (J.prog_intro_strictness jp)) ->
+    binds c "$vcontext" (L.value_object ptr) ->
+    concl_ext_expr_resvalue BR jst jc c st st' r 
+        (J.spec_binding_inst J.codetype_global None jp []) (fun jrv => jrv = J.resvalue_empty).
+Proof.
+    introv Hlred Hcinv Hinv Hbinds1 Hbinds2.
+    asserts_rewrite 
+        (concat (List.map E.js_element_to_func (J.prog_elements jp)) = E.prog_funcs (E.js_prog_to_ejs jp)) in Hlred.
+    { destruct jp. reflexivity. }
+    rewrite E.js_funcdecl_to_func_lemma in Hlred.
+    lets Hvenv : execution_ctx_related_variable_env (context_invariant_execution_ctx_related Hcinv) Hbinds2.
+    inverts Hvenv as Hf3 Hf4 Hlerel Hvenveq. symmetry in Hvenveq.
+    repeat ljs_autoforward.
+    forwards_th : binding_inst_function_decls_lemma; try prove_bag.
+    destr_concl; try ljs_handle_abort.
+    res_related_invert.
+    repeat ljs_autoforward.
+    forwards_th: has_binding_lemma. prove_bag.
+    destr_concl; try ljs_handle_abort.
+    res_related_invert.
+    resvalue_related_invert.
+    repeat ljs_autoforward.
+    forwards_th : binding_inst_var_decls_lemma; try prove_bag.
+    destr_concl; try ljs_handle_abort.
+    res_related_invert.
+    resvalue_related_only_invert.
+    repeat ljs_autoforward.
+    jauto_js 15.
+Qed.
+
+Lemma binding_inst_eval_lemma : forall BR k jst jc c st st' r ptr jp,
+    L.red_exprh k c st (L.expr_basic
+          (E.init_bindings_prog true E.make_fobj (concat (List.map E.js_element_to_func (J.prog_elements jp))) 
+              (J.prog_vardecl jp))) (L.out_ter st' r) ->
+    context_invariant BR jc c ->
+    state_invariant BR jst st ->
+    binds c "$strict" (L.value_bool (J.prog_intro_strictness jp)) ->
+    binds c "$vcontext" (L.value_object ptr) ->
+    concl_ext_expr_resvalue BR jst jc c st st' r 
+        (J.spec_binding_inst J.codetype_eval None jp []) (fun jrv => jrv = J.resvalue_empty).
+Proof.
+    introv Hlred Hcinv Hinv Hbinds1 Hbinds2.
+    asserts_rewrite 
+        (concat (List.map E.js_element_to_func (J.prog_elements jp)) = E.prog_funcs (E.js_prog_to_ejs jp)) in Hlred.
+    { destruct jp. reflexivity. }
+    rewrite E.js_funcdecl_to_func_lemma in Hlred.
+    lets Hvenv : execution_ctx_related_variable_env (context_invariant_execution_ctx_related Hcinv) Hbinds2.
+    inverts Hvenv as Hf3 Hf4 Hlerel Hvenveq. symmetry in Hvenveq.
+    repeat ljs_autoforward.
+    forwards_th : binding_inst_function_decls_lemma; try prove_bag.
+    destr_concl; try ljs_handle_abort.
+    res_related_invert.
+    repeat ljs_autoforward.
+    forwards_th: has_binding_lemma. prove_bag.
+    destr_concl; try ljs_handle_abort.
+    res_related_invert.
+    resvalue_related_invert.
+    repeat ljs_autoforward.
+    forwards_th : binding_inst_var_decls_lemma; try prove_bag.
+    destr_concl; try ljs_handle_abort.
+    res_related_invert.
+    resvalue_related_only_invert.
+    repeat ljs_autoforward.
+    jauto_js 15.
+Qed.
+
+Lemma binding_inst_func_lemma : forall BR k jst jc c st st' r ptr ptr1 ptr2 jptr jp jvs vs is,
+    L.red_exprh k c st (L.expr_basic
+          (E.init_bindings_func E.make_fobj is (concat (List.map E.js_element_to_func (J.prog_elements jp))) 
+              (J.prog_vardecl jp))) (L.out_ter st' r) ->
+    context_invariant BR jc c ->
+    state_invariant BR jst st ->
+    values_related BR jvs vs ->
+    binds c "obj" (L.value_object ptr) ->
+    binds c "$strict" (L.value_bool (J.prog_intro_strictness jp)) ->
+    binds c "$vcontext" (L.value_object ptr2) ->
+    binds c "args" (L.value_object ptr1) ->
+    fact_iarray ptr1 vs \in BR ->
+    fact_js_obj jptr ptr \in BR ->
+    J.object_method J.object_formal_parameters_ jst jptr (Some is) ->
+    concl_ext_expr_resvalue BR jst jc c st st' r 
+        (J.spec_binding_inst J.codetype_func (Some jptr) jp jvs) (fun jrv => jrv = J.resvalue_empty).
+Proof.
+    introv Hlred Hcinv Hinv Hvrels Hbinds1 Hbinds2 Hbinds3 Hbinds4.
+    introv Hf1 Hf2 Hom.
+    asserts_rewrite 
+        (concat (List.map E.js_element_to_func (J.prog_elements jp)) = E.prog_funcs (E.js_prog_to_ejs jp)) in Hlred.
+    { destruct jp. reflexivity. }
+    rewrite E.js_funcdecl_to_func_lemma in Hlred.
+    lets Hvenv : execution_ctx_related_variable_env (context_invariant_execution_ctx_related Hcinv) Hbinds3.
+    inverts Hvenv as Hf3 Hf4 Hlerel Hvenveq. symmetry in Hvenveq.
+    repeat ljs_autoforward.
+    forwards_th : binding_inst_formal_params_lemma; try prove_bag.
+    destr_concl; try ljs_handle_abort.
+    res_related_invert.
+    repeat ljs_autoforward.
+    forwards_th : binding_inst_function_decls_lemma; try prove_bag.
+    destr_concl; try ljs_handle_abort.
+    res_related_invert.
+    repeat ljs_autoforward.
+    unfolds E.init_args_obj.
+    inverts red_exprh H16. (* TODO *)
+    ljs_apply.
+    ljs_context_invariant_after_apply.
+    repeat ljs_autoforward.
+    cases_decide; [idtac | repeat inv_ljs].
+    repeat ljs_autoforward.
+    forwards_th: has_binding_lemma. prove_bag.
+    destr_concl; try ljs_handle_abort.
+    res_related_invert.
+    resvalue_related_invert.
+    destruct b. { (* has binding named "arguments" *)
+        repeat ljs_autoforward.
+        forwards_th : binding_inst_var_decls_lemma; try prove_bag.
+        destr_concl; try ljs_handle_abort.
+        res_related_invert.
+        repeat ljs_autoforward.
+        jauto_js 15.
+    } { (* no binding named "arguments" *)
+        repeat ljs_autoforward.
+        forwards_th : binding_inst_arg_obj_lemma; try prove_bag. eauto_js. eauto_js.
+        destr_concl; try ljs_handle_abort.
+        res_related_invert.
+        resvalue_related_only_invert.
+        repeat ljs_autoforward.
+        forwards_th : binding_inst_var_decls_lemma; try prove_bag.
+        destr_concl; try ljs_handle_abort.
+        res_related_invert.
+        repeat ljs_autoforward.
+        jauto_js 15.
+    }
+Qed.
+
+Opaque E.init_bindings_func.
+
+Lemma call_lemma : forall BR k jst jc c st st' r jfb is jle v v1 vs ptr ptr1 jptr jv1 jvs,
+    ih_stat k ->
+    ih_call k ->
+    L.red_exprh k c st (L.expr_app_2 v [L.value_object ptr; v1; L.value_object ptr1]) (L.out_ter st' r) ->
+    context_invariant BR jc c ->
+    state_invariant BR jst st ->
+    usercode_related BR jfb is jle v ->
+    value_related BR jv1 v1 ->
+    values_related BR jvs vs ->
+    fact_iarray ptr1 vs \in BR ->
+    fact_js_obj jptr ptr \in BR ->
+    J.object_method J.object_scope_ jst jptr (Some jle) ->
+    J.object_method J.object_formal_parameters_ jst jptr (Some is) ->
+    J.object_method J.object_code_ jst jptr (Some jfb) ->
+    concl_ext_expr_value BR jst jc c st st' r 
+        (J.spec_entering_func_code_3 jptr jvs (J.funcbody_is_strict jfb) jfb jv1 (J.spec_call_default_1 jptr)) 
+        (fun jv => True).
+Proof.
+    introv IHt IHc Hlred Hcinv Hinv Hucrel Hvrel Hvrels Hbs Hbs1.
+    introv Hom1 Hom2 Hom3.
+    inverts Hucrel as Huci.
+    unfolds funcbody_closure. unfolds funcbody_expr. unfolds E.make_lambda_expr.
+    cases_let as Hprog.
+    inverts red_exprh Hlred.
+    ljs_apply.
+    subst c'.
+    repeat ljs_autoforward.
+    lets Hlerel : usercode_context_invariant_lexical_env_related Huci ___; try eassumption.
+    forwards_th Hx : usercode_context_invariant_restore; try eassumption. 
+    destruct_hyp Hx.
+    repeat ljs_autoforward.
+    rewrite <- (js_prog_intro_eta jp) in Hprog.
+    simpl in Hprog.
+    injects Hprog.
+    rewrite js_prog_intro_eta in *.
+    lets Hstrict : usercode_context_invariant_has_strict Huci. (* TODO do a lemma *)
+    rewrite index_binds_eq in Hstrict. destruct_hyp Hstrict.
+    lets Hstreq : usercode_context_invariant_strict Huci Hstrict. subst_hyp Hstreq.
+    forwards_th : binding_inst_func_lemma; try prove_bag 8. { eauto_js. } skip. (* TODO state consistency *)
+    destr_concl; try ljs_handle_abort.
+    res_related_invert.
+    resvalue_related_only_invert.
+    repeat ljs_autoforward.
+    asserts Hom3' : (J.object_method J.object_code_ jst' jptr (Some (J.funcbody_intro jp s))). 
+        skip. (* TODO state consistency *)
+    lets [Hfbe|Hfbe] : classic (J.funcbody_empty (J.funcbody_intro jp s)). { 
+        (* special case required by the spec *)
+        unfolds J.funcbody_empty. unfolds J.prog_empty.
+        simpl in Hfbe. rewrite Hfbe in *.
+        repeat ljs_autoforward.
+        jauto_js 10.
+    }
+    forwards_th Hx : prog_ok_call_lemma.
+    destruct_hyp Hx. (* TODO destr_concl *)
+    res_related_invert; repeat ljs_autoforward. { (* normal exit *)
+        jauto_js 10.
+    } { (* exception *)
+        jauto_js 10.
+    } { (* return *)
+        jauto_js 10.
+    } { (* break *)
+        (* TODO: should never happen due to syntax constraints, but unable to prove this now. *)
+        skip. 
+    } { (* continue *)
+        (* TODO: should never happen due to syntax constraints, but unable to prove this now. *)
+        skip. 
+    }
+Qed.
+
+Lemma red_spec_call_prealloc_ok : forall k jpre, th_call_prealloc k jpre.
+Proof.
+    introv Hcinv Hinv Hvrel Hf Hrel Hvrels Hlred.
+    destruct jpre.
+    + skip.
+    + skip.
+    + skip.
+    + skip.
+    + skip.
+    + skip.
+    + skip.
+    + skip.
+    + skip.
+    + skip.
+    + skip.
+    + skip.
+    + skip.
+    + skip.
+    + skip.
+    + skip.
+    + skip.
+    + skip.
+    + skip.
+    + skip.
+    + skip.
+    + skip.
+    + skip.
+    + skip.
+    + skip.
+    + skip.
+    + skip.
+    + skip.
+    + skip.
+    + skip.
+    + skip.
+    + skip.
+    + skip.
+    + skip.
+    + skip.
+    + skip.
+    + skip.
+    + skip.
+    + skip.
+    + skip.
+    + skip.
+    + skip.
+    + skip.
+    + skip.
+    + skip.
+    + skip.
+    + skip.
+    + skip.
+    + skip.
+    + skip.
+    + skip.
+    + skip.
+    + skip.
+    + skip.
+    + skip.
+    + skip.
+    + skip.
+    + skip.
+    + skip.
+    + skip.
+    + skip.
+    + skip.
+    + skip.
+Qed.
+
+Lemma red_spec_call_ok : forall k,
+    ih_stat k ->
+    ih_call k ->
+    th_call k.
+Proof.
+    introv IHt IHc Hcinv Hinv Hvrel Halo Hbs Hvrels Hlred. 
+    ljs_invert_apply.
+    repeat ljs_autoforward.
+    inverts red_exprh H7. (* TODO *)
+    lets (jcon&Hmeth&Hcall) : object_method_call_some_lemma Hinv Hbs ___; try eassumption.
+    inverts Hcall. { (* prealloc *)
+        forwards_th Hx : red_spec_call_prealloc_ok; try eassumption. 
+        destr_concl; try ljs_handle_abort.
+        jauto_js.
+    } { (* default *)
+        ljs_invert_apply.
+        repeat ljs_autoforward.
+        lets (jfb&is&jle&Hmcode&Hparams&Hscope&Hcode) : object_method_code_some_lemma ___; try eassumption.
+        lets (str&Heqstr&Hfbstr) : object_strict_lemma ___; try eassumption.
+        subst_hyp Heqstr.
+        ljs_invert_apply.
+        repeat ljs_autoforward.
+        symmetry in Hfbstr.
+        destruct str. { (* strict *)
+            repeat ljs_autoforward.
+            forwards_th Hcl : call_lemma; try eassumption.
+            rewrite <- Hfbstr in Hcl.
+            destr_concl; try ljs_handle_abort.
+            jauto_js 15.
+        } { (* not strict *)
+            do 2 inv_fwd_ljs.
+            (* TODO better condition handling *)
+            ljs_out_redh_ter.
+            ljs_bool_red_exprh; repeat determine_epsilon.
+            cases_isTrue as Hevcond. { (* null or undefined *)
+                repeat ljs_autoforward.
+                rewrite case_classic_l_eq in Hevcond.
+                asserts Hmycond : (jv = J.value_prim J.prim_null \/ jv = J.value_prim J.prim_undef). {
+                    inverts Hvrel;
+                    destruct Hevcond as [Hevcond|Hevcond]; inverts Hevcond; eauto_js.
+                }
+                forwards_th Hcl : call_lemma; try eassumption.
+                rewrite <- Hfbstr in Hcl.
+                destr_concl; try ljs_handle_abort.
+                jauto_js 15.
+            } 
+            repeat ljs_autoforward.
+            cases_decide as Hisobj. { (* is object *)
+                repeat ljs_autoforward.
+                inverts Hvrel; inverts Hisobj.
+                forwards_th Hcl : call_lemma; try eassumption.
+                rewrite <- Hfbstr in Hcl.
+                destr_concl; try ljs_handle_abort.
+                jauto_js 15.
+            } { (* not object *)
+                rewrite case_classic_l_eq in Hevcond.
+                rew_logic in Hevcond. destruct Hevcond as (Hevcond1&Hevcond2).
+                asserts Hmycond : (jv <> JsSyntax.value_prim JsSyntax.prim_null /\
+                    jv <> JsSyntax.value_prim JsSyntax.prim_undef /\
+                    JsPreliminary.type_of jv <> JsSyntax.type_object). {
+                    inverts Hvrel; try solve [false; eauto_js]; eauto_js.
+                }
+                repeat ljs_autoforward.
+                forwards_th : red_spec_to_object_ok.
+                destr_concl; try ljs_handle_abort.
+                res_related_invert.
+                resvalue_related_invert.
+                repeat ljs_autoforward.
+                forwards_th Hcl : call_lemma; try eauto_js. skip. skip. skip. (* TODO state consistency issue! *)
+                rewrite <- Hfbstr in Hcl.
+                destr_concl; try ljs_handle_abort.
+                jauto_js 15.
+            }
+        }
+    } { (* bind *)
+        skip. (* TODO *) (* NOT YET IN JSCERT *)
+    }
+Qed.
