LambdaS5/coq/LjsRulesCorrectSpecFuns.v
@@ -788,16 +788,16 @@ Proof.
             inverts Hacc.
             inverts Hgop1 as Harel. inverts Harel.
             repeat ljs_autoforward. simpls.
-            jauto_js 30.
+            jauto_set_slim; eauto_js 20. eauto_js. (* TODO *)
         } { (* is data *)
             inverts Hgop1 as Harel; try solve [false; apply Hacc; eapply L.is_accessor_accessor]. inverts Harel.
             repeat ljs_autoforward. simpls.
-            jauto_js 21.
+            jauto_set_slim; eauto_js 20. eauto_js. (* TODO *)
         }
     } { (* not found *)
         forwards Hgop : object_method_get_own_property_default_not_index_lemma; try eassumption.
         repeat ljs_autoforward.
-        jauto_js 20.
+        jauto_set_slim; eauto_js 20. eauto_js. (* TODO *)
     }
 Qed.
 
@@ -859,12 +859,12 @@ Proof.
             unfolds L.object_proto. rewrite Heq1 in *.
             forwards_th Hx : IH. math. prove_bag.
             destruct_hyp Hx; try ljs_handle_abort;
-            jauto_js 30.
+            jauto_set_slim; eauto_js 20. (* TODO *)
         }
     } { (* found data *)
-        jauto_js 30.
+        jauto_set_slim; eauto_js 20. (* TODO *)
     } { (* found accessor *)
-        jauto_js 30.
+        jauto_set_slim; eauto_js 20. (* TODO *)
     }
 Qed.
 
@@ -880,9 +880,7 @@ Proof.
     intro k.
     induction_wf IH : lt_wf k.
     introv Hlred Hcinv Hinv Hf.
-    inverts red_exprh Hlred.
-    ljs_apply.
-    ljs_context_invariant_after_apply.
+    ljs_invert_apply.
     forwards : object_method_get_property_lemma; try eassumption.
     forwards : object_method_get_own_property_lemma; try eassumption.
     repeat ljs_autoforward.
@@ -2121,147 +2119,6 @@ Proof.
     }
 Qed.
 
-Lemma binding_inst_formal_params_lemma_lemma : forall BR k jst jc c st st' r is vs jvs1 jvs2 ptr ptr1 jeptr b k',
-    L.red_exprh k c st (L.expr_basic (L.expr_seqs_then L.expr_empty
-            (map E.init_arg (zipl_stream (LibStream.map string_of_nat (nat_stream_from k')) is)))) 
-        (L.out_ter st' r) ->
-    context_invariant BR jc c ->
-    state_invariant BR jst st ->
-    values_related BR (jvs1 ++ jvs2) vs ->
-    k' = length jvs1 /\ length jvs2 > 0 \/ k' >= length jvs1 /\ jvs2 = [] ->
-    binds c "$strict" (L.value_bool b) ->
-    binds c "$vcontext" (L.value_object ptr) ->
-    binds c "args" (L.value_object ptr1) ->
-    fact_iarray ptr1 vs \in BR ->
-    fact_js_env jeptr ptr \in BR ->
-    concl_ext_expr_resvalue BR jst jc c st st' r 
-        (J.spec_binding_inst_formal_params jvs2 jeptr is b) (fun jrv => jrv = J.resvalue_empty).    
-Proof.
-    introv.
-    unfolds E.init_args.
-    inductions is gen BR k jst st jvs1 jvs2;
-    introv Hlred Hcinv Hinv Hvrels Hk' Hbinds1 Hbinds2 Hbinds3 Hf1 Hf2. {
-        repeat ljs_autoforward.
-        jauto_js 10.
-    }
-    simpl in Hlred.
-    rew_map in Hlred.
-    repeat ljs_autoforward.
-    forwards_th Harridx : array_idx_lemma. reflexivity. eassumption. eassumption.
-    destruct Harridx as (?&Heq1&jv&v&Heq2&Hvrel&Harridx). subst_hyp Heq1. subst_hyp Heq2.
-    asserts Hjvs2 : (k' >= length jvs1 /\ jvs2 = [] /\ v = L.value_undefined /\ jv = J.value_prim J.prim_undef \/ 
-            k' = length jvs1 /\ exists jvs2', jvs2 = jv::jvs2'). {
-        destruct Hk' as [(Hk1&Hk2)|(Hk1&Hk2)]. {
-            right. split. assumption. 
-            destruct jvs2; rew_length in Hk2; try solve [false; math].
-            destruct Harridx as [Harridx|Harridx]. {
-                erewrite <- values_related_length_lemma in Harridx by eassumption.
-                rew_length in Harridx. destruct_hyp Harridx. false. math.
-            }
-            destruct Harridx as (Harridx1&Harridx2).
-            apply Nth_app_inv in Harridx1.
-            destruct Harridx1 as [Harridx1|Harridx1]. {
-                apply Nth_lt_length in Harridx1. false. math.
-            }
-            destruct Harridx1 as (k''&Heqk''&Harridx1).
-            asserts Hzero : (k'' = 0). { math. } subst_hyp Hzero.
-            inverts Harridx1.
-            jauto.
-        } {
-            left. 
-            destruct Harridx as [Harridx|Harridx]. {
-                destruct_hyp Harridx. jauto.
-            }
-            subst_hyp Hk2.
-            destruct Harridx as (Harridx1&Harridx2).
-            rew_app in Harridx1.
-            apply Nth_lt_length in Harridx1. false. math.
-        }
-    }
-    clear Harridx. clear Hk'.
-    asserts Hexit : (exists jvs1' jvs2', values_related BR (jvs1' ++ jvs2') vs /\
-            (S k' = length jvs1' /\ length jvs2' > 0 \/ S k' >= length jvs1' /\ jvs2' = []) /\
-            (k' >= length jvs1 /\ jvs2 = [] /\ v = L.value_undefined /\ jv = J.value_prim J.prim_undef /\
-                jvs1' = jvs1 /\ jvs2' = jvs2 \/ 
-             k' = length jvs1 /\ jvs1' = jvs1 & jv /\ jvs2 = jv::jvs2')). {
-        destruct Hjvs2 as [Hjvs2|Hjvs2]. {
-            exists jvs1 jvs2.
-            destruct_hyp Hjvs2. splits. 
-            + assumption. 
-            + right. split. math. reflexivity.
-            + left. jauto_js.
-        } {
-            destruct_hyp Hjvs2. destruct jvs2' as [|jv' jvs2']. {
-                exists (jvs1&jv) (@nil J.value). splits.
-                + rew_app. assumption.
-                + right. split. { rew_length. math. } reflexivity.
-                + right. jauto_js.
-            }
-            exists (jvs1&jv) (jv'::jvs2'). splits. 
-            + rew_app. assumption.
-            + left. split. { rew_length. math. } { rew_length. math. }
-            + right. jauto_js.
-        }
-    }
-    repeat ljs_autoforward.
-    inverts red_exprh H3. (* TODO *)
-    ljs_apply.
-    ljs_context_invariant_after_apply.
-    repeat ljs_autoforward.
-    forwards_th: has_binding_lemma. prove_bag.
-    destr_concl; [idtac | destruct_hyp Hjvs2; try ljs_handle_abort].
-    res_related_invert.
-    resvalue_related_invert.
-    repeat ljs_autoforward.
-    destruct b0. { (* binding already exists *)
-        repeat ljs_autoforward.
-        forwards_th: set_mutable_binding_lemma. prove_bag.
-        destr_concl; [idtac | destruct_hyp Hjvs2; try ljs_handle_abort].
-        res_related_invert.
-        resvalue_related_only_invert.
-        repeat ljs_autoforward.
-        destruct Hexit as (jvs1'&jvs2'&Hvrels'&Hsk'&Hjvs2').
-        forwards_th Hx : IHis; try prove_bag. eauto_js.
-        destr_concl; [idtac | destruct_hyp Hjvs2'; try ljs_handle_abort].
-        destruct_hyp Hjvs2'; jauto_js 10.
-    } { (* binding does not exist *)
-        repeat ljs_autoforward.
-        forwards_th: create_mutable_binding_lemma_none. prove_bag.
-        destr_concl; [idtac | destruct_hyp Hjvs2; try ljs_handle_abort].
-        res_related_invert.
-        resvalue_related_only_invert.
-        repeat ljs_autoforward.
-        forwards_th: set_mutable_binding_lemma. prove_bag.
-        destr_concl; [idtac | destruct_hyp Hjvs2; try ljs_handle_abort]. 
-        res_related_invert.
-        resvalue_related_only_invert.
-        repeat ljs_autoforward.
-        destruct Hexit as (jvs1'&jvs2'&Hvrels'&Hsk'&Hjvs2').
-        forwards_th Hx : IHis; try prove_bag. eauto_js.
-        destr_concl; [idtac | destruct_hyp Hjvs2'; try ljs_handle_abort].
-        destruct_hyp Hjvs2'; jauto_js 10.
-    }
-Qed.
-
-Lemma binding_inst_formal_params_lemma : forall BR k jst jc c st st' r is vs jvs ptr ptr1 jeptr b,
-    L.red_exprh k c st (L.expr_basic (E.init_args is)) (L.out_ter st' r) ->
-    context_invariant BR jc c ->
-    state_invariant BR jst st ->
-    values_related BR jvs vs ->
-    binds c "$strict" (L.value_bool b) ->
-    binds c "$vcontext" (L.value_object ptr) ->
-    binds c "args" (L.value_object ptr1) ->
-    fact_iarray ptr1 vs \in BR ->
-    fact_js_env jeptr ptr \in BR ->
-    concl_ext_expr_resvalue BR jst jc c st st' r 
-        (J.spec_binding_inst_formal_params jvs jeptr is b) (fun jrv => jrv = J.resvalue_empty).    
-Proof.
-    introv Hlred Hcinv Hinv Hvrels Hbinds1 Hbinds2 Hbinds3 Hf1 Hf2.
-    asserts Hvrels' : (values_related BR ([]++jvs) vs). { rew_app. assumption. }
-    forwards_th : binding_inst_formal_params_lemma_lemma; try prove_bag.
-    destruct jvs; rew_length; intuition math.
-Qed.
-
 (* TODO move *)
 Lemma red_spec_creating_function_object_ok : forall BR k jst jc c' c st st' r is s jp jle,
     L.red_exprh k c st
@@ -2346,326 +2203,6 @@ Lemma create_arguments_object_ok : forall BR k jst jc c st st' r jptr ptr ptr1 p
 Proof.
 Admitted. (* TODO *)
 
-Lemma binding_inst_arg_obj_lemma : forall BR k jst jc c st st' r jptr ptr ptr1 ptr2(*ptr3*)is jvs vs jeptr jlenv v b,
-    L.red_exprh k c st (L.expr_app_2 LjsInitEnv.privEnvDefineArgsObjOk
-        [L.value_object ptr2; L.value_null(*object ptr3*); L.value_object ptr1; L.value_object ptr; L.value_bool b]) 
-        (L.out_ter st' r) ->
-    context_invariant BR jc c ->
-    state_invariant BR jst st ->
-    values_related BR jvs vs ->
-    lexical_env_related BR jlenv v ->
-    fact_js_obj jptr ptr \in BR ->
-    fact_iarray ptr1 vs \in BR ->
-(*    fact_iarray ptr3 (map L.value_string is) \in BR -> TODO non-strict args obj *)
-    fact_js_env jeptr ptr2 \in BR ->
-    fact_ctx_parent ptr2 v \in BR ->
-    J.execution_ctx_variable_env jc = jeptr::jlenv ->
-    concl_ext_expr_resvalue BR jst jc c st st' r 
-        (J.spec_binding_inst_arg_obj jptr is jvs jeptr b) (fun jrv => jrv = J.resvalue_empty).
-Proof.
-    introv Hlred Hcinv Hinv Hvrel Hlrel Hf1 Hf2 Hf3 Hf4 Hvenv.
-    inverts red_exprh Hlred.
-    ljs_apply.
-    ljs_context_invariant_after_apply.
-    repeat ljs_autoforward.
-    forwards_th Hx : create_arguments_object_ok; try prove_bag.
-    rewrite <- Hvenv in Hx.
-    destr_concl; try ljs_handle_abort.
-    res_related_invert.
-    resvalue_related_only_invert.
-    repeat ljs_autoforward.
-    destruct b. { (* strict *)
-        repeat ljs_autoforward.
-        forwards_th : create_immutable_binding_lemma. prove_bag.
-        destr_concl; try ljs_handle_abort.
-        res_related_invert.
-        repeat ljs_autoforward.
-        forwards_th : initialize_immutable_binding_lemma. prove_bag.
-        destr_concl; try ljs_handle_abort.
-        res_related_invert.
-        resvalue_related_only_invert.
-        jauto_js 10.
-    } { (* non-strict *)
-        repeat ljs_autoforward.
-        forwards_th : create_set_mutable_binding_lemma_none. prove_bag.
-        destr_concl; try ljs_handle_abort.
-        res_related_invert.
-        resvalue_related_only_invert.
-        jauto_js 10.
-    }
-Qed.
-
-Lemma binding_inst_function_decls_lemma : forall BR k jst jc c st st' r jfds jeptr ptr b1 b2,
-    L.red_exprh k c st (L.expr_basic 
-        (E.init_funcs b1 E.make_fobj (map E.js_funcdecl_to_func jfds))) (L.out_ter st' r) ->
-    context_invariant BR jc c ->
-    state_invariant BR jst st ->
-    binds c "$strict" (L.value_bool b2) ->
-    binds c "$vcontext" (L.value_object ptr) ->
-    fact_js_env jeptr ptr \in BR ->
-    concl_ext_expr_resvalue BR jst jc c st st' r 
-        (J.spec_binding_inst_function_decls jeptr jfds b2 b1) (fun jrv => jrv = J.resvalue_empty).    
-Proof.
-    introv.
-    unfolds E.init_funcs.
-    inductions jfds gen BR k jst st;
-    introv Hlred Hcinv Hinv Hbinds1 Hbinds2 Hf. {
-        repeat ljs_autoforward.
-        jauto_js.
-    }
-    destruct a. destruct funcdecl_body.
-    rew_map in Hlred.
-    repeat ljs_autoforward.
-    rewrite exprjs_prog_strictness_eq in *.
-    forwards_th : red_spec_creating_function_object_ok. skip. (* { TODO in ES5 variable env required, fixed in ES6
-        introv Hbinds.
-        binds_inv.
-        applys (execution_ctx_related_lexical_env (context_invariant_execution_ctx_related Hcinv)).
-        assumption.
-    } *)
-    destr_concl; try ljs_handle_abort.
-    res_related_invert.
-    resvalue_related_invert.
-    repeat ljs_autoforward.
-    inverts red_exprh H12. (* TODO *)
-    ljs_apply.
-    ljs_context_invariant_after_apply.
-    repeat ljs_autoforward.
-    forwards_th: has_binding_lemma. prove_bag.
-    destr_concl; try ljs_handle_abort.
-    res_related_invert.
-    resvalue_related_invert.
-    repeat ljs_autoforward.
-    destruct b. { (* binding already exists *)
-        repeat ljs_autoforward.
-        cases_decide as Hgctx. { (* on global context *)
-            skip. (* TODO global context *)
-        }
-        asserts Hq : (jeptr <> J.env_loc_global_env_record). {
-            unfolds LjsInitEnv.privglobalContext.
-            rewrite stx_eq_object_eq_lemma in Hgctx.
-            forwards Hger : context_invariant_global_env_record_lemma Hcinv.
-            intro Hjeptr. subst_hyp Hjeptr. apply Hgctx.
-            determine_fact_js_env.
-            reflexivity.
-        }
-        repeat ljs_autoforward.
-        forwards_th: set_mutable_binding_lemma. prove_bag.
-        destr_concl; try ljs_handle_abort.
-        res_related_invert.
-        repeat ljs_autoforward.
-        forwards_th : IHjfds; try prove_bag.
-        destr_concl; try ljs_handle_abort.
-        res_related_invert.
-        jauto_js 10.
-    } { (* binding does not exist *)
-        repeat ljs_autoforward.
-        forwards_th: create_mutable_binding_lemma_some. prove_bag.
-        destr_concl; try ljs_handle_abort.
-        res_related_invert.
-        repeat ljs_autoforward.
-        forwards_th: set_mutable_binding_lemma. prove_bag.
-        destr_concl; try ljs_handle_abort.
-        res_related_invert.
-        resvalue_related_only_invert.
-        repeat ljs_autoforward.
-        forwards_th : IHjfds; try prove_bag.
-        destr_concl; try ljs_handle_abort.
-        res_related_invert.
-        jauto_js 10.
-    }
-Qed.
-
-Lemma binding_inst_var_decls_lemma : forall BR k jst jc c st st' r is jeptr ptr b1 b2,
-    L.red_exprh k c st (L.expr_basic (E.init_vars b1 is)) (L.out_ter st' r) ->
-    context_invariant BR jc c ->
-    state_invariant BR jst st ->
-    binds c "$strict" (L.value_bool b2) ->
-    binds c "$vcontext" (L.value_object ptr) ->
-    fact_js_env jeptr ptr \in BR ->
-    concl_ext_expr_resvalue BR jst jc c st st' r 
-        (J.spec_binding_inst_var_decls jeptr is b1 b2) (fun jrv => jrv = J.resvalue_empty).
-Proof.
-    introv.
-    unfolds E.init_vars.
-    inductions is gen BR k jst st;
-    introv Hlred Hcinv Hinv Hbinds1 Hbinds2 Hf. {
-        repeat ljs_autoforward.
-        jauto_js.
-    }
-    rew_map in Hlred.
-    repeat ljs_autoforward.
-    inverts red_exprh H3.
-    ljs_apply.
-    ljs_context_invariant_after_apply.
-    repeat ljs_autoforward.
-    forwards_th: has_binding_lemma. eassumption.
-    destr_concl; try ljs_handle_abort.
-    res_related_invert.
-    resvalue_related_invert.
-    repeat ljs_autoforward.
-    destruct b. { (* binding already exists *)
-        repeat ljs_autoforward.
-        forwards_th : IHis; try prove_bag.
-        destr_concl; try ljs_handle_abort.
-        res_related_invert.
-        jauto_js 10.
-    } { (* binding does not exist *)
-        repeat ljs_autoforward.
-        forwards_th: create_set_mutable_binding_lemma_some. prove_bag.
-        destr_concl; try ljs_handle_abort.
-        res_related_invert.
-        repeat ljs_autoforward.
-        forwards_th : IHis; try prove_bag.
-        destr_concl; try ljs_handle_abort.
-        res_related_invert.
-        jauto_js 10.
-    }
-Qed.
-
-Opaque E.init_args E.init_vars E.init_funcs.
-
-Lemma binding_inst_global_lemma : forall BR k jst jc c st st' r ptr jp,
-    L.red_exprh k c st (L.expr_basic
-          (E.init_bindings_prog false E.make_fobj (concat (List.map E.js_element_to_func (J.prog_elements jp))) 
-              (J.prog_vardecl jp))) (L.out_ter st' r) ->
-    context_invariant BR jc c ->
-    state_invariant BR jst st ->
-    binds c "$strict" (L.value_bool (J.prog_intro_strictness jp)) ->
-    binds c "$vcontext" (L.value_object ptr) ->
-    concl_ext_expr_resvalue BR jst jc c st st' r 
-        (J.spec_binding_inst J.codetype_global None jp []) (fun jrv => jrv = J.resvalue_empty).
-Proof.
-    introv Hlred Hcinv Hinv Hbinds1 Hbinds2.
-    asserts_rewrite 
-        (concat (List.map E.js_element_to_func (J.prog_elements jp)) = E.prog_funcs (E.js_prog_to_ejs jp)) in Hlred.
-    { destruct jp. reflexivity. }
-    rewrite E.js_funcdecl_to_func_lemma in Hlred.
-    lets Hvenv : execution_ctx_related_variable_env (context_invariant_execution_ctx_related Hcinv) Hbinds2.
-    inverts Hvenv as Hf3 Hf4 Hlerel Hvenveq. symmetry in Hvenveq.
-    repeat ljs_autoforward.
-    forwards_th : binding_inst_function_decls_lemma; try prove_bag.
-    destr_concl; try ljs_handle_abort.
-    res_related_invert.
-    repeat ljs_autoforward.
-    forwards_th: has_binding_lemma. prove_bag.
-    destr_concl; try ljs_handle_abort.
-    res_related_invert.
-    resvalue_related_invert.
-    repeat ljs_autoforward.
-    forwards_th : binding_inst_var_decls_lemma; try prove_bag.
-    destr_concl; try ljs_handle_abort.
-    res_related_invert.
-    resvalue_related_only_invert.
-    repeat ljs_autoforward.
-    jauto_js 15.
-Qed.
-
-Lemma binding_inst_eval_lemma : forall BR k jst jc c st st' r ptr jp,
-    L.red_exprh k c st (L.expr_basic
-          (E.init_bindings_prog true E.make_fobj (concat (List.map E.js_element_to_func (J.prog_elements jp))) 
-              (J.prog_vardecl jp))) (L.out_ter st' r) ->
-    context_invariant BR jc c ->
-    state_invariant BR jst st ->
-    binds c "$strict" (L.value_bool (J.prog_intro_strictness jp)) ->
-    binds c "$vcontext" (L.value_object ptr) ->
-    concl_ext_expr_resvalue BR jst jc c st st' r 
-        (J.spec_binding_inst J.codetype_eval None jp []) (fun jrv => jrv = J.resvalue_empty).
-Proof.
-    introv Hlred Hcinv Hinv Hbinds1 Hbinds2.
-    asserts_rewrite 
-        (concat (List.map E.js_element_to_func (J.prog_elements jp)) = E.prog_funcs (E.js_prog_to_ejs jp)) in Hlred.
-    { destruct jp. reflexivity. }
-    rewrite E.js_funcdecl_to_func_lemma in Hlred.
-    lets Hvenv : execution_ctx_related_variable_env (context_invariant_execution_ctx_related Hcinv) Hbinds2.
-    inverts Hvenv as Hf3 Hf4 Hlerel Hvenveq. symmetry in Hvenveq.
-    repeat ljs_autoforward.
-    forwards_th : binding_inst_function_decls_lemma; try prove_bag.
-    destr_concl; try ljs_handle_abort.
-    res_related_invert.
-    repeat ljs_autoforward.
-    forwards_th: has_binding_lemma. prove_bag.
-    destr_concl; try ljs_handle_abort.
-    res_related_invert.
-    resvalue_related_invert.
-    repeat ljs_autoforward.
-    forwards_th : binding_inst_var_decls_lemma; try prove_bag.
-    destr_concl; try ljs_handle_abort.
-    res_related_invert.
-    resvalue_related_only_invert.
-    repeat ljs_autoforward.
-    jauto_js 15.
-Qed.
-
-Lemma binding_inst_func_lemma : forall BR k jst jc c st st' r ptr ptr1 ptr2 jptr jp jvs vs is,
-    L.red_exprh k c st (L.expr_basic
-          (E.init_bindings_func E.make_fobj is (concat (List.map E.js_element_to_func (J.prog_elements jp))) 
-              (J.prog_vardecl jp))) (L.out_ter st' r) ->
-    context_invariant BR jc c ->
-    state_invariant BR jst st ->
-    values_related BR jvs vs ->
-    binds c "obj" (L.value_object ptr) ->
-    binds c "$strict" (L.value_bool (J.prog_intro_strictness jp)) ->
-    binds c "$vcontext" (L.value_object ptr2) ->
-    binds c "args" (L.value_object ptr1) ->
-    fact_iarray ptr1 vs \in BR ->
-    fact_js_obj jptr ptr \in BR ->
-    J.object_method J.object_formal_parameters_ jst jptr (Some is) ->
-    concl_ext_expr_resvalue BR jst jc c st st' r 
-        (J.spec_binding_inst J.codetype_func (Some jptr) jp jvs) (fun jrv => jrv = J.resvalue_empty).
-Proof.
-    introv Hlred Hcinv Hinv Hvrels Hbinds1 Hbinds2 Hbinds3 Hbinds4.
-    introv Hf1 Hf2 Hom.
-    asserts_rewrite 
-        (concat (List.map E.js_element_to_func (J.prog_elements jp)) = E.prog_funcs (E.js_prog_to_ejs jp)) in Hlred.
-    { destruct jp. reflexivity. }
-    rewrite E.js_funcdecl_to_func_lemma in Hlred.
-    lets Hvenv : execution_ctx_related_variable_env (context_invariant_execution_ctx_related Hcinv) Hbinds3.
-    inverts Hvenv as Hf3 Hf4 Hlerel Hvenveq. symmetry in Hvenveq.
-    repeat ljs_autoforward.
-    forwards_th : binding_inst_formal_params_lemma; try prove_bag.
-    destr_concl; try ljs_handle_abort.
-    res_related_invert.
-    repeat ljs_autoforward.
-    forwards_th : binding_inst_function_decls_lemma; try prove_bag.
-    destr_concl; try ljs_handle_abort.
-    res_related_invert.
-    repeat ljs_autoforward.
-    unfolds E.init_args_obj.
-    inverts red_exprh H16. (* TODO *)
-    ljs_apply.
-    ljs_context_invariant_after_apply.
-    repeat ljs_autoforward.
-    cases_decide; [idtac | repeat inv_ljs].
-    repeat ljs_autoforward.
-    forwards_th: has_binding_lemma. prove_bag.
-    destr_concl; try ljs_handle_abort.
-    res_related_invert.
-    resvalue_related_invert.
-    destruct b. { (* has binding named "arguments" *)
-        repeat ljs_autoforward.
-        forwards_th : binding_inst_var_decls_lemma; try prove_bag.
-        destr_concl; try ljs_handle_abort.
-        res_related_invert.
-        repeat ljs_autoforward.
-        jauto_js 15.
-    } { (* no binding named "arguments" *)
-        repeat ljs_autoforward.
-        forwards_th : binding_inst_arg_obj_lemma; try prove_bag. eauto_js. eauto_js.
-        destr_concl; try ljs_handle_abort.
-        res_related_invert.
-        resvalue_related_only_invert.
-        repeat ljs_autoforward.
-        forwards_th : binding_inst_var_decls_lemma; try prove_bag.
-        destr_concl; try ljs_handle_abort.
-        res_related_invert.
-        repeat ljs_autoforward.
-        jauto_js 15.
-    }
-Qed.
-
-Opaque E.init_bindings_func.
-
 (* TODO move *)
 Hint Constructors J.red_prog : js_ljs.
 
@@ -2733,167 +2270,31 @@ Proof.
     intros. destruct jp. eapply prog_ok_lemma; eassumption.
 Qed.
 
-Lemma call_lemma : forall BR k jst jc c st st' r jfb is jle v v1 vs ptr ptr1 jptr jv1 jvs,
-    ih_stat k ->
-    ih_call_prealloc k ->
-    L.red_exprh k c st (L.expr_app_2 v [L.value_object ptr; v1; L.value_object ptr1]) (L.out_ter st' r) ->
-    context_invariant BR jc c ->
-    state_invariant BR jst st ->
-    usercode_related BR jfb is jle v ->
-    value_related BR jv1 v1 ->
-    values_related BR jvs vs ->
-    fact_iarray ptr1 vs \in BR ->
-    fact_js_obj jptr ptr \in BR ->
-    J.object_method J.object_scope_ jst jptr (Some jle) ->
-    J.object_method J.object_formal_parameters_ jst jptr (Some is) ->
-    J.object_method J.object_code_ jst jptr (Some jfb) ->
-    concl_ext_expr_value BR jst jc c st st' r 
-        (J.spec_entering_func_code_3 jptr jvs (J.funcbody_is_strict jfb) jfb jv1 (J.spec_call_default_1 jptr)) 
-        (fun jv => True).
-Proof.
-    introv IHt IHp Hlred Hcinv Hinv Hucrel Hvrel Hvrels Hbs Hbs1.
-    introv Hom1 Hom2 Hom3.
-    inverts Hucrel as Huci.
-    unfolds funcbody_closure. unfolds funcbody_expr. unfolds E.make_lambda_expr.
-    cases_let as Hprog.
-    inverts red_exprh Hlred.
-    ljs_apply.
-    subst c'.
-    repeat ljs_autoforward.
-    lets Hlerel : usercode_context_invariant_lexical_env_related Huci ___; try eassumption.
-    forwards_th Hx : usercode_context_invariant_restore; try eassumption. 
-    destruct_hyp Hx.
-    repeat ljs_autoforward.
-    rewrite <- (js_prog_intro_eta jp) in Hprog.
-    simpl in Hprog.
-    injects Hprog.
-    rewrite js_prog_intro_eta in *.
-    lets Hstrict : usercode_context_invariant_has_strict Huci. (* TODO do a lemma *)
-    rewrite index_binds_eq in Hstrict. destruct_hyp Hstrict.
-    lets Hstreq : usercode_context_invariant_strict Huci Hstrict. subst_hyp Hstreq.
-    forwards_th : binding_inst_func_lemma; try prove_bag 8. { eauto_js. } skip. (* TODO state consistency *)
-    destr_concl; try ljs_handle_abort.
-    res_related_invert.
-    resvalue_related_only_invert.
-    repeat ljs_autoforward.
-    asserts Hom3' : (J.object_method J.object_code_ jst' jptr (Some (J.funcbody_intro jp s))). 
-        skip. (* TODO state consistency *)
-    lets [Hfbe|Hfbe] : classic (J.funcbody_empty (J.funcbody_intro jp s)). { 
-        (* special case required by the spec *)
-        unfolds J.funcbody_empty. unfolds J.prog_empty.
-        simpl in Hfbe. rewrite Hfbe in *.
-        repeat ljs_autoforward.
-        jauto_js 10.
-    }
-    forwards_th Hx : prog_ok_call_lemma.
-    destruct_hyp Hx. (* TODO destr_concl *)
-    res_related_invert; repeat ljs_autoforward. { (* normal exit *)
-        jauto_js 10.
-    } { (* exception *)
-        jauto_js 10.
-    } { (* return *)
-        jauto_js 10.
-    } { (* break *)
-        (* TODO: should never happen due to syntax constraints, but unable to prove this now. *)
-        skip. 
-    } { (* continue *)
-        (* TODO: should never happen due to syntax constraints, but unable to prove this now. *)
-        skip. 
-    }
-Qed.
-
-Lemma red_spec_call_ok : forall BR k jst jc c st st' ptr v ptr1 vs r jptr jv jvs,
-    ih_stat k ->
-    ih_call_prealloc k ->
-    L.red_exprh k c st 
-        (L.expr_app_2 LjsInitEnv.privAppExpr [L.value_object ptr; v; L.value_object ptr1]) 
-        (L.out_ter st' r) ->
-    context_invariant BR jc c ->
-    state_invariant BR jst st ->
-    value_related BR jv v ->
-    values_related BR jvs vs ->
-    fact_iarray ptr1 vs \in BR ->
-    fact_js_obj jptr ptr \in BR ->
-    concl_ext_expr_value BR jst jc c st st' r (J.spec_call jptr jv jvs) (fun jv => True).
-Proof.
-    introv IHt IHp Hlred Hcinv Hinv Hvrel Hvrels Halo Hbs. 
-    ljs_invert_apply.
-    repeat ljs_autoforward.
-    inverts red_exprh H7. (* TODO *)
-    lets (jcon&Hmeth&Hcall) : object_method_call_some_lemma Hinv Hbs ___; try eassumption.
-    inverts Hcall. { (* prealloc *)
-        forwards Hx : IHp; [idtac |  
-        forwards_th Hxx : Hx]; try eassumption. omega. (* TODO *)
-        destr_concl; try ljs_handle_abort.
-        jauto_js.
-    } { (* default *)
-        ljs_invert_apply.
-        repeat ljs_autoforward.
-        lets (jfb&is&jle&Hmcode&Hparams&Hscope&Hcode) : object_method_code_some_lemma ___; try eassumption.
-        lets (str&Heqstr&Hfbstr) : object_strict_lemma ___; try eassumption.
-        subst_hyp Heqstr.
-        ljs_invert_apply.
-        repeat ljs_autoforward.
-        symmetry in Hfbstr.
-        destruct str. { (* strict *)
-            repeat ljs_autoforward.
-            forwards_th Hcl : call_lemma; try eassumption.
-            rewrite <- Hfbstr in Hcl.
-            destr_concl; try ljs_handle_abort.
-            jauto_js 15.
-        } { (* not strict *)
-            do 2 inv_fwd_ljs.
-            (* TODO better condition handling *)
-            ljs_out_redh_ter.
-            ljs_bool_red_exprh; repeat determine_epsilon.
-            cases_isTrue as Hevcond. { (* null or undefined *)
-                repeat ljs_autoforward.
-                rewrite case_classic_l_eq in Hevcond.
-                asserts Hmycond : (jv = J.value_prim J.prim_null \/ jv = J.value_prim J.prim_undef). {
-                    inverts Hvrel;
-                    destruct Hevcond as [Hevcond|Hevcond]; inverts Hevcond; eauto_js.
-                }
-                forwards_th Hcl : call_lemma; try eassumption.
-                rewrite <- Hfbstr in Hcl.
-                destr_concl; try ljs_handle_abort.
-                jauto_js 15.
-            } 
-            repeat ljs_autoforward.
-            cases_decide as Hisobj. { (* is object *)
-                repeat ljs_autoforward.
-                inverts Hvrel; inverts Hisobj.
-                forwards_th Hcl : call_lemma; try eassumption.
-                rewrite <- Hfbstr in Hcl.
-                destr_concl; try ljs_handle_abort.
-                jauto_js 15.
-            } { (* not object *)
-                rewrite case_classic_l_eq in Hevcond.
-                rew_logic in Hevcond. destruct Hevcond as (Hevcond1&Hevcond2).
-                asserts Hmycond : (jv <> JsSyntax.value_prim JsSyntax.prim_null /\
-                    jv <> JsSyntax.value_prim JsSyntax.prim_undef /\
-                    JsPreliminary.type_of jv <> JsSyntax.type_object). {
-                    inverts Hvrel; try solve [false; eauto_js]; eauto_js.
-                }
-                repeat ljs_autoforward.
-                forwards_th : red_spec_to_object_ok.
-                destr_concl; try ljs_handle_abort.
-                res_related_invert.
-                resvalue_related_invert.
-                repeat ljs_autoforward.
-                forwards_th Hcl : call_lemma; try eauto_js. skip. skip. skip. (* TODO state consistency issue! *)
-                rewrite <- Hfbstr in Hcl.
-                destr_concl; try ljs_handle_abort.
-                jauto_js 15.
-            }
-        }
-    } { (* bind *)
-        skip. (* TODO *) (* NOT YET IN JSCERT *)
-    }
-Qed.
+(* TODO move to common *)
+Ltac apply_ih_call := match goal with
+    | H : ih_call ?k', 
+      HS : state_invariant ?BR ?jst ?st,
+      HC' : context_invariant ?BR' ?jc ?c', 
+      HR : L.red_exprh ?k ?c ?st (L.expr_app_2 LjsInitEnv.privAppExpr _) _ |- _ =>
+        let Hle := fresh "Hle" in
+        let HC := fresh "HC" in
+        let Hsec := fresh "Hsec" in
+        let Hsub := fresh "H" in
+        asserts Hle : (k < k')%nat; [math | idtac];
+        asserts Hsub : (BR' \c BR); [prove_bag | idtac];
+        asserts HC : (context_invariant BR jc c); 
+            [applys context_invariant_bisim_incl_preserved Hsub; ljs_context_invariant | idtac]; 
+        lets Hih : H Hle HC HS HR; 
+        [eauto_js
+        |prove_bag|prove_bag
+        |try repeat first [eapply Forall2_nil | eapply Forall2_cons; [eauto_js | idtac]]
+        |clear Hle; clear Hsub; clear HS; clear HR; clear HC]
+   (*     lets Hsec : L.red_exprh_state_security_ok HR;  *)
+    end.
 
 Lemma get_default_lemma : forall BR k jst jc c st st' r ptr jptr v jv s,
     ih_stat k ->
-    ih_call_prealloc k ->
+    ih_call k ->
     L.red_exprh k c st (L.expr_app_2 LjsInitEnv.privGet [L.value_object ptr; v; L.value_string s])
         (L.out_ter st' r) ->
     context_invariant BR jc c ->
@@ -2902,7 +2303,7 @@ Lemma get_default_lemma : forall BR k jst jc c st st' r ptr jptr v jv s,
     value_related BR jv v ->
     concl_ext_expr_value BR jst jc c st st' r (J.spec_object_get_1 J.builtin_get_default jv jptr s) (fun _ => True).
 Proof.
-    introv IHt IHp Hlred Hcinv Hinv Hf Hvrel.
+    introv IHt IHc Hlred Hcinv Hinv Hf Hvrel.
     ljs_invert_apply.
     repeat ljs_autoforward.
     forwards_th Hx : get_property_lemma. eassumption.
@@ -2929,7 +2330,7 @@ Proof.
             forwards_th Hy : zero_arg_obj_lemma.
             destruct_hyp Hy.
             repeat ljs_autoforward.
-            forwards_th : red_spec_call_ok. eapply Forall2_nil. prove_bag. prove_bag.
+            apply_ih_call.
             destr_concl; try ljs_handle_abort.
             jauto_js.
         }
@@ -2938,7 +2339,7 @@ Qed.
 
 Lemma get_1_lemma : forall BR k jst jc c st st' r ptr jptr v jv s x,
     ih_stat k ->
-    ih_call_prealloc k ->
+    ih_call k ->
     L.red_exprh k c st (L.expr_app_2 LjsInitEnv.privGet [L.value_object ptr; v; L.value_string s])
         (L.out_ter st' r) ->
     context_invariant BR jc c ->
@@ -2948,7 +2349,7 @@ Lemma get_1_lemma : forall BR k jst jc c st st' r ptr jptr v jv s x,
     J.object_method J.object_get_ jst jptr x ->
     concl_ext_expr_value BR jst jc c st st' r (J.spec_object_get_1 x jv jptr s) (fun _ => True).
 Proof.
-    introv IHt IHp Hlred Hcinv Hinv Hf Hvrel Hm.
+    introv IHt IHc Hlred Hcinv Hinv Hf Hvrel Hm.
     forwards Hmm : object_method_get_lemma; try eassumption. (* TODO *)
     asserts Heq : (x = J.builtin_get_default). skip. (* TODO exotic objects *) subst_hyp Heq.
     forwards_th : get_default_lemma. eassumption.
@@ -2958,7 +2359,7 @@ Qed.
 
 Lemma get_lemma : forall BR k jst jc c st st' r ptr jptr s,
     ih_stat k ->
-    ih_call_prealloc k ->
+    ih_call k ->
     L.red_exprh k c st (L.expr_app_2 LjsInitEnv.privGet1 [L.value_object ptr; L.value_string s])
         (L.out_ter st' r) ->
     context_invariant BR jc c ->
@@ -2966,7 +2367,7 @@ Lemma get_lemma : forall BR k jst jc c st st' r ptr jptr s,
     fact_js_obj jptr ptr \in BR ->
     concl_ext_expr_value BR jst jc c st st' r (J.spec_object_get jptr s) (fun _ => True).
 Proof.
-    introv IHt IHp Hlred Hcinv Hinv Hf.
+    introv IHt IHc Hlred Hcinv Hinv Hf.
     ljs_invert_apply.
     forwards Hmm : object_method_get_lemma; try eassumption. (* TODO *)
     repeat ljs_autoforward.
@@ -2977,7 +2378,7 @@ Qed.
 
 Lemma get_prim_lemma : forall BR k jst jc c st st' r v jv s,
     ih_stat k ->
-    ih_call_prealloc k ->
+    ih_call k ->
     L.red_exprh k c st (L.expr_app_2 LjsInitEnv.privGetPrim [v; L.value_string s])
         (L.out_ter st' r) ->
     context_invariant BR jc c ->
@@ -2985,7 +2386,7 @@ Lemma get_prim_lemma : forall BR k jst jc c st st' r v jv s,
     value_related BR jv v ->
     concl_ext_expr_value BR jst jc c st st' r (J.spec_prim_value_get jv s) (fun _ => True).
 Proof.
-    introv IHt IHp Hlred Hcinv Hinv Hvrel.
+    introv IHt IHc Hlred Hcinv Hinv Hvrel.
     ljs_invert_apply.
     repeat ljs_autoforward.
     forwards_th : red_spec_to_object_ok.
@@ -3038,7 +2439,7 @@ Qed.
 
 Lemma put_default_lemma : forall BR k jst jc c st st' r ptr jptr v jv v1 jv1 s b,
     ih_stat k ->
-    ih_call_prealloc k ->
+    ih_call k ->
     L.red_exprh k c st (L.expr_app_2 LjsInitEnv.privPut 
         [L.value_object ptr; v; L.value_string s; v1; L.value_bool b]) (L.out_ter st' r) ->
     context_invariant BR jc c ->
@@ -3049,7 +2450,7 @@ Lemma put_default_lemma : forall BR k jst jc c st st' r ptr jptr v jv v1 jv1 s b
     concl_ext_expr_resvalue BR jst jc c st st' r (J.spec_object_put_1 J.builtin_put_default jv jptr s jv1 b) 
         (fun jrv => jrv = J.resvalue_empty).
 Proof.
-    introv IHt IHp Hlred Hcinv Hinv Hf Hvrel1 Hvrel2.
+    introv IHt IHc Hlred Hcinv Hinv Hf Hvrel1 Hvrel2.
     ljs_invert_apply.
     forwards Hcp : object_method_can_put_lemma; try eassumption.
     forwards Hgp : object_method_get_property_lemma; try eassumption.
@@ -3107,7 +2508,7 @@ Proof.
             forwards_th Hy : one_arg_obj_lemma.
             destruct_hyp Hy.
             repeat ljs_autoforward.
-            forwards_th : red_spec_call_ok; try prove_bag. eapply Forall2_cons. eauto_js. eapply Forall2_nil.
+            apply_ih_call.
             destr_concl; try ljs_handle_abort.
             res_related_invert.
             resvalue_related_only_invert.
@@ -3375,7 +2776,7 @@ Admitted.
 
 Lemma red_spec_construct_ok : forall BR k jst jc c st st' ptr ptr1 vs r jptr jvs,
     ih_stat k ->
-    ih_call_prealloc k ->
+    ih_call k ->
     L.red_exprh k c st 
         (L.expr_app_2 LjsInitEnv.privrunConstruct [L.value_object ptr; L.value_object ptr1]) 
         (L.out_ter st' r) ->
@@ -3386,7 +2787,7 @@ Lemma red_spec_construct_ok : forall BR k jst jc c st st' ptr ptr1 vs r jptr jvs
     fact_js_obj jptr ptr \in BR ->
     concl_ext_expr_value BR jst jc c st st' r (J.spec_construct jptr jvs) (fun jv => True).
 Proof.
-    introv IHt IHp Hlred Hcinv Hinv Hvrels Halo Hbs.
+    introv IHt IHc Hlred Hcinv Hinv Hvrels Halo Hbs.
     inverts red_exprh Hlred.
     ljs_apply.
     ljs_context_invariant_after_apply.
